code/experimental/curve25519/Hacl.Spec.Curve25519.Field64.fst
@@ -264,20 +264,14 @@ let subtract_p4 (f0, f1, f2, f3) =
   // assert_norm (0xffffffffffffffff = pow2 64 - 1);
   // assert_norm (0xffffffffffffffed = pow2 64 - 19);
 
-  let mask0 = uint64_eq_mask f3 (u64 0x7fffffffffffffff) in
-  let mask1 = mask0 &. uint64_eq_mask f2 (u64 0xffffffffffffffff) in
-  let mask2 = mask1 &. uint64_eq_mask f1 (u64 0xffffffffffffffff) in
-  let mask = mask2 &. uint64_gte_mask f0 (u64 0xffffffffffffffed) in
-
-  let p0 = mask &. u64 0xffffffffffffffed in
-  let p1 = mask &. u64 0xffffffffffffffff in
-  let p2 = mask &. u64 0xffffffffffffffff in
-  let p3 = mask &. u64 0x7fffffffffffffff in
-
-  let f0' = f0 -. p0 in
-  let f1' = f1 -. p1 in
-  let f2' = f2 -. p2 in
-  let f3' = f3 -. p3 in
-
+  let m0 = uint64_gte_mask f0 (u64 0xffffffffffffffed) in
+  let m1 = uint64_eq_mask f1 (u64 0xffffffffffffffff) in
+  let m2 = uint64_eq_mask f2 (u64 0xffffffffffffffff) in
+  let m3 = uint64_eq_mask f3 (u64 0x7fffffffffffffff) in
+  let mask = m0 &. m1 &. m2 &. m3 in
+  let f0' = f0 -. (mask &. u64 0xffffffffffffffed) in
+  let f1' = f1 -. (mask &. u64 0xffffffffffffffff) in
+  let f2' = f2 -. (mask &. u64 0xffffffffffffffff) in
+  let f3' = f3 -. (mask &. u64 0x7fffffffffffffff) in
   lemma_subtract_p (f0, f1, f2, f3) (f0', f1', f2', f3');
   (f0', f1', f2', f3')
