code/experimental/curve25519/lemmas/Hacl.Spec.Curve25519.Field51.Lemmas.fst
@@ -484,6 +484,8 @@ let lemma_carry5_simplify c0 c1 c2 c3 c4 t0 t1 t2 t3 t4 =
     v t4 * pow51 * pow51 * pow51 * pow51)
    (v c4 * 19) prime
 
+#set-options "--z3rlimit 100 --max_fuel 1"
+
 val lemma_smul_felem5:
     #m1:scale64
   -> #m2:scale64_5
@@ -495,8 +497,6 @@ val lemma_smul_felem5:
       v u1 * v f24 * pow51 * pow51 * pow51 * pow51)
 let lemma_smul_felem5 #m1 #m2 u1 f2 =
   let (f20, f21, f22, f23, f24) = f2 in
-  assert (v u1 * as_nat5 f2 == v u1 * (v f20 + v f21 * pow51 + v f22 * pow51 * pow51 +
-    v f23 * pow51 * pow51 * pow51 + v f24 * pow51 * pow51 * pow51 * pow51));
   lemma_mul5_distr_l (v u1) (v f20) (v f21 * pow51) (v f22 * pow51 * pow51)
     (v f23 * pow51 * pow51 * pow51) (v f24 * pow51 * pow51 * pow51 * pow51)
 
@@ -519,11 +519,6 @@ val lemma_smul_add_felem5:
 let lemma_smul_add_felem5 #m1 #m2 #m3 u1 f2 acc1 =
   let (f20, f21, f22, f23, f24) = f2 in
   let (o0, o1, o2, o3, o4) = acc1 in
-  assert (wide_as_nat5 acc1 + uint_v u1 * as_nat5 f2 ==
-    v o0 + v o1 * pow51 + v o2 * pow51 * pow51 +
-    v o3 * pow51 * pow51 * pow51 + v o4 * pow51 * pow51 * pow51 * pow51 +
-    v u1 * (v f20 + v f21 * pow51 + v f22 * pow51 * pow51 +
-    v f23 * pow51 * pow51 * pow51 + v f24 * pow51 * pow51 * pow51 * pow51));
   lemma_mul5_distr_l (v u1) (v f20) (v f21 * pow51) (v f22 * pow51 * pow51)
     (v f23 * pow51 * pow51 * pow51) (v f24 * pow51 * pow51 * pow51 * pow51)
 
@@ -690,3 +685,196 @@ let lemma_load_felem u64s =
   let f = (f0, f1, f2, f3, f4) in
   lemma_load_felem_fits5 f u64s;
   lemma_load_felem5 f u64s
+
+val lemma_subtract_p5_0:
+    f:felem5{felem_fits5 f (1, 1, 1, 1, 1)}
+  -> f':felem5
+  -> Lemma
+    (requires (
+      let (f0, f1, f2, f3, f4) = f in
+      let (f0', f1', f2', f3', f4') = f' in
+     (v f4 <> 0x7ffffffffffff || v f3 <> 0x7ffffffffffff || v f2 <> 0x7ffffffffffff || v f1 <> 0x7ffffffffffff || v f0 < 0x7ffffffffffed) /\
+      (v f0' = v f0 && v f1' = v f1 && v f2' = v f2 && v f3' = v f3 && v f4' = v f4)))
+    (ensures as_nat5 f' == as_nat5 f % prime)
+let lemma_subtract_p5_0 f f' =
+  let (f0, f1, f2, f3, f4) = f in
+  let (f0', f1', f2', f3', f4') = f' in
+  assert_norm (0x7ffffffffffff = pow2 51 - 1);
+  assert_norm (0x7ffffffffffed = pow2 51 - 19);
+  assert_norm (pow51 = pow2 51);
+  assert (as_nat5 f == v f0 + v f1 * pow51 + v f2 * pow51 * pow51 +
+    v f3 * pow51 * pow51 * pow51 + v f4 * pow51 * pow51 * pow51 * pow51);
+  assert (as_nat5 f <= pow2 51 - 20 + (pow2 51 - 1) * pow2 51 + (pow2 51 - 1) * pow2 51 * pow2 51 +
+    (pow2 51 - 1) * pow2 51 * pow2 51 * pow2 51 + (pow2 51 - 1) * pow2 51 * pow2 51 * pow2 51 * pow2 51);
+  assert (as_nat5 f < pow2 255 - 19);
+  assert (as_nat5 f == as_nat5 f');
+  FStar.Math.Lemmas.modulo_lemma (as_nat5 f') prime
+
+val lemma_subtract_p5_1:
+    f:felem5{felem_fits5 f (1, 1, 1, 1, 1)}
+  -> f':felem5
+  -> Lemma
+    (requires (
+      let (f0, f1, f2, f3, f4) = f in
+      let (f0', f1', f2', f3', f4') = f' in
+     (v f4 = 0x7ffffffffffff && v f3 = 0x7ffffffffffff && v f2 = 0x7ffffffffffff && v f1 = 0x7ffffffffffff && v f0 >= 0x7ffffffffffed) /\
+      (v f0' = v f0 - 0x7ffffffffffed && v f1' = v f1 - 0x7ffffffffffff && v f2' = v f2 - 0x7ffffffffffff &&
+       v f3' = v f3 - 0x7ffffffffffff && v f4' = v f4 - 0x7ffffffffffff)))
+    (ensures as_nat5 f' == as_nat5 f % prime)
+let lemma_subtract_p5_1 f f' =
+  let (f0, f1, f2, f3, f4) = f in
+  let (f0', f1', f2', f3', f4') = f' in
+  assert_norm (0x7ffffffffffff = pow2 51 - 1);
+  assert_norm (0x7ffffffffffed = pow2 51 - 19);
+  assert_norm (pow51 = pow2 51);
+  assert (as_nat5 f' % prime == (v f0' + v f1' * pow51 + v f2' * pow51 * pow51 +
+    v f3' * pow51 * pow51 * pow51 + v f4' * pow51 * pow51 * pow51 * pow51) % prime);
+  assert (as_nat5 f' % prime ==
+    (v f0 - (pow2 51 - 19) + (v f1 - (pow2 51 - 1)) * pow2 51 + (v f2 - (pow2 51 - 1)) * pow2 51 * pow2 51 +
+    (v f3 - (pow2 51 - 1)) * pow2 51 * pow2 51 * pow2 51 +
+    (v f4 - (pow2 51 - 1)) * pow2 51 * pow2 51 * pow2 51 * pow2 51) % prime);
+  assert (as_nat5 f' % prime ==
+    (v f0 + v f1 * pow2 51 + v f2 * pow2 51 * pow2 51 +
+    v f3 * pow2 51 * pow2 51 * pow2 51 + v f4 * pow2 51 * pow2 51 * pow2 51 * pow2 51 - prime) % prime);
+  FStar.Math.Lemmas.lemma_mod_sub (as_nat5 f) 1 prime
+
+val lemma_subtract_p:
+    f:felem5{felem_fits5 f (1, 1, 1, 1, 1)}
+  -> f':felem5
+  -> Lemma
+    (requires (
+      let (f0, f1, f2, f3, f4) = f in
+      let (f0', f1', f2', f3', f4') = f' in
+     (((v f4 <> 0x7ffffffffffff || v f3 <> 0x7ffffffffffff || v f2 <> 0x7ffffffffffff || v f1 <> 0x7ffffffffffff || v f0 < 0x7ffffffffffed) /\
+      (v f0' = v f0 && v f1' = v f1 && v f2' = v f2 && v f3' = v f3 && v f4' = v f4)) \/
+     ((v f4 = 0x7ffffffffffff && v f3 = 0x7ffffffffffff && v f2 = 0x7ffffffffffff && v f1 = 0x7ffffffffffff && v f0 >= 0x7ffffffffffed) /\
+      (v f0' = v f0 - 0x7ffffffffffed && v f1' = v f1 - 0x7ffffffffffff && v f2' = v f2 - 0x7ffffffffffff &&
+       v f3' = v f3 - 0x7ffffffffffff && v f4' = v f4 - 0x7ffffffffffff)))))
+    (ensures as_nat5 f' == as_nat5 f % prime)
+let lemma_subtract_p f f' =
+  let (f0, f1, f2, f3, f4) = f in
+  let (f0', f1', f2', f3', f4') = f' in
+  if ((v f4 <> 0x7ffffffffffff || v f3 <> 0x7ffffffffffff || v f2 <> 0x7ffffffffffff || v f1 <> 0x7ffffffffffff || v f0 < 0x7ffffffffffed) &&
+      (v f0' = v f0 && v f1' = v f1 && v f2' = v f2 && v f3' = v f3 && v f4' = v f4))
+  then lemma_subtract_p5_0 f f'
+  else lemma_subtract_p5_1 f f'
+
+val lemma_store_felem1: f:felem5{felem_fits5 f (1, 1, 1, 1, 1) /\ as_nat5 f < prime} ->
+  Lemma (
+    let (f0, f1, f2, f3, f4) = f in
+    v f0 + (v f1 % pow2 13) * pow2 51 +
+    (v f1 / pow2 13 + (v f2 % pow2 26) * pow2 38) * pow2 64 +
+    (v f2 / pow2 26 + (v f3 % pow2 39) * pow2 25) * pow2 128 +
+    (v f3 / pow2 39 + v f4 * pow2 12) * pow2 192 == as_nat5 f)
+let lemma_store_felem1 f =
+  let (f0, f1, f2, f3, f4) = f in
+  assert_norm (pow51 = pow2 51);
+  assert_norm (pow2 38 * pow2 64 = pow2 102);
+  assert_norm (pow2 25 * pow2 128 = pow2 153);
+  assert_norm (pow2 12 * pow2 192 = pow2 204);
+  assert (
+    v f0 + (v f1 % pow2 13) * pow2 51 +
+    (v f1 / pow2 13 + (v f2 % pow2 26) * pow2 38) * pow2 64 +
+    (v f2 / pow2 26 + (v f3 % pow2 39) * pow2 25) * pow2 128 +
+    (v f3 / pow2 39 + v f4 * pow2 12) * pow2 192 ==
+    v f0 + (v f1 % pow2 13) * pow2 51 +
+    v f1 / pow2 13 * pow2 64 + (v f2 % pow2 26) * pow2 102 +
+    v f2 / pow2 26 * pow2 128 + (v f3 % pow2 39) * pow2 153 +
+    v f3 / pow2 39 * pow2 192 + v f4 * pow2 204);
+  assert_norm (pow2 64 = pow2 13 * pow2 51);
+  FStar.Math.Lemmas.euclidean_division_definition (v f1) (pow2 13);
+
+  assert_norm (pow2 102 = pow2 51 * pow2 51);
+  assert_norm (pow2 128 = pow2 26 * pow2 51 * pow2 51);
+  FStar.Math.Lemmas.euclidean_division_definition (v f2) (pow2 26);
+
+  assert_norm (pow2 153 = pow2 51 * pow2 51 * pow2 51);
+  assert_norm (pow2 192 = pow2 39 * pow2 51 * pow2 51 * pow2 51);
+  FStar.Math.Lemmas.euclidean_division_definition (v f3) (pow2 39)
+
+val lemma_store_felem0: f:felem5{felem_fits5 f (1, 1, 1, 1, 1) /\ as_nat5 f < prime} ->
+  Lemma (
+    let (f0, f1, f2, f3, f4) = f in
+    let o0 = v f0 + (v f1 % pow2 13) * pow2 51 in
+    let o1 = v f1 / pow2 13 + (v f2 % pow2 26) * pow2 38 in
+    let o2 = v f2 / pow2 26 + (v f3 % pow2 39) * pow2 25 in
+    let o3 = v f3 / pow2 39 + (v f4 % pow2 52) * pow2 12 in
+    as_nat5 f == o0 + o1 * pow2 64 + o2 * pow2 64 * pow2 64 + o3 * pow2 64 * pow2 64 * pow2 64)
+let lemma_store_felem0 f =
+  assert_norm (pow51 = pow2 51);
+  let (f0, f1, f2, f3, f4) = f in
+  let o0 = v f0 + (v f1 % pow2 13) * pow2 51 in
+  let o1 = v f1 / pow2 13 + (v f2 % pow2 26) * pow2 38 in
+  let o2 = v f2 / pow2 26 + (v f3 % pow2 39) * pow2 25 in
+  let o3 = v f3 / pow2 39 + (v f4 % pow2 52) * pow2 12 in
+  assert (v f4 % pow2 52 = v f4);
+  assert (
+    o0 + o1 * pow2 64 + o2 * pow2 64 * pow2 64 + o3 * pow2 64 * pow2 64 * pow2 64 ==
+    v f0 + (v f1 % pow2 13) * pow2 51 +
+    (v f1 / pow2 13 + (v f2 % pow2 26) * pow2 38) * pow2 64 +
+    (v f2 / pow2 26 + (v f3 % pow2 39) * pow2 25) * pow2 64 * pow2 64 +
+    (v f3 / pow2 39 + v f4 * pow2 12) * pow2 64 * pow2 64 * pow2 64);
+  assert_norm (pow2 64 * pow2 64 = pow2 128);
+  assert_norm (pow2 64 * pow2 64 * pow2 64 = pow2 192);
+  assert (
+    o0 + o1 * pow2 64 + o2 * pow2 64 * pow2 64 + o3 * pow2 64 * pow2 64 * pow2 64 ==
+    v f0 + (v f1 % pow2 13) * pow2 51 +
+    (v f1 / pow2 13 + (v f2 % pow2 26) * pow2 38) * pow2 64 +
+    (v f2 / pow2 26 + (v f3 % pow2 39) * pow2 25) * pow2 128 +
+    (v f3 / pow2 39 + v f4 * pow2 12) * pow2 192);
+  lemma_store_felem1 f
+
+val lemma_store_felem: f:felem5{felem_fits5 f (1, 1, 1, 1, 1) /\ as_nat5 f < prime} ->
+  Lemma (
+    let (f0, f1, f2, f3, f4) = f in
+    let o0 = f0 |. (f1 <<. 51ul) in
+    let o1 = (f1 >>. 13ul) |. (f2 <<. 38ul) in
+    let o2 = (f2 >>. 26ul) |. (f3 <<. 25ul) in
+    let o3 = (f3 >>. 39ul) |. (f4 <<. 12ul) in
+    as_nat5 f == v o0 + v o1 * pow2 64 + v o2 * pow2 64 * pow2 64 + v o3 * pow2 64 * pow2 64 * pow2 64)
+let lemma_store_felem f =
+  let (f0, f1, f2, f3, f4) = f in
+  assert_norm (pow51 = pow2 51);
+  let o0 = f0 |. (f1 <<. 51ul) in
+  //assert (v (f1 <<. 51ul) == (v f1 * pow2 51) % pow2 64);
+  FStar.Math.Lemmas.pow2_multiplication_modulo_lemma_2 (v f1) 64 51;
+  //assert (v (f1 <<. 51ul) == (v f1 % pow2 13) * pow2 51);
+  logor_disjoint64 f0 (f1 <<. 51ul) 51;
+  //assert (v o0 == v f0 + (v f1 % pow2 13) * pow2 51);
+
+  let o1 = (f1 >>. 13ul) |. (f2 <<. 38ul) in
+  //assert (v (f1 >>. 13ul) == v f1 / pow2 13);
+  FStar.Math.Lemmas.lemma_div_lt (v f1) 51 13;
+  //assert (v f1 / pow2 13 < pow2 38);
+
+  //assert (v (f2 <<. 38ul) == (v f2 * pow2 38) % pow2 64);
+  FStar.Math.Lemmas.pow2_multiplication_modulo_lemma_2 (v f2) 64 38;
+  //assert (v (f2 <<. 38ul) == (v f2 % pow2 26) * pow2 38);
+  FStar.Math.Lemmas.multiple_modulo_lemma (v f2 % pow2 26) (pow2 38);
+  logor_disjoint64 (f1 >>. 13ul) (f2 <<. 38ul) 38;
+  //assert (v o1 == v f1 / pow2 13 + (v f2 % pow2 26) * pow2 38);
+
+  let o2 = (f2 >>. 26ul) |. (f3 <<. 25ul) in
+  //assert (v (f2 >>. 26ul) == v f2 / pow2 26);
+  FStar.Math.Lemmas.lemma_div_lt (v f2) 51 26;
+  //assert (v f2 / pow2 26 < pow2 25);
+
+  //assert (v (f3 <<. 25ul) == (v f3 * pow2 25) % pow2 64);
+  FStar.Math.Lemmas.pow2_multiplication_modulo_lemma_2 (v f3) 64 25;
+  //assert (v (f3 <<. 25ul) == (v f3 % pow2 39) * pow2 25);
+  FStar.Math.Lemmas.multiple_modulo_lemma (v f3 % pow2 39) (pow2 25);
+  logor_disjoint64 (f2 >>. 26ul) (f3 <<. 25ul) 25;
+  //assert (v o2 == v f2 / pow2 26 + (v f3 % pow2 39) * pow2 25);
+
+  let o3 = (f3 >>. 39ul) |. (f4 <<. 12ul) in
+  //assert (v (f3 >>. 39ul) == v f3 / pow2 39);
+  FStar.Math.Lemmas.lemma_div_lt (v f3) 51 39;
+  //assert (v f3 / pow2 39 < pow2 12);
+
+  //assert (v (f4 <<. 12ul) == (v f4 * pow2 12) % pow2 64);
+  FStar.Math.Lemmas.pow2_multiplication_modulo_lemma_2 (v f4) 64 12;
+  //assert (v (f4 <<. 12ul) == (v f4 % pow2 52) * pow2 12);
+  FStar.Math.Lemmas.multiple_modulo_lemma (v f4 % pow2 52) (pow2 12);
+  logor_disjoint64 (f3 >>. 39ul) (f4 <<. 12ul) 12;
+  //assert (v o3 == v f3 / pow2 39 + (v f4 % pow2 52) * pow2 12);
+  lemma_store_felem0 f
